fixup classes: Avoid soundness issue with raw pointers + unreachable panic

Source/DafnyCore/GeneratedFromDafny/DCOMP.cs
@@ -754,12 +754,24 @@ namespace DCOMP {
         return RAST.__default.ObjectType(underlying);
       }
     }
+    public Dafny.ISequence<Dafny.Rune> UnreachablePanicIfVerified(Dafny.ISequence<Dafny.Rune> optText) {
+      if (((this).ObjectType).is_RawPointers) {
+        return Dafny.Sequence<Dafny.Rune>.UnicodeFromString("unsafe { ::std::hint::unreachable_unchecked() }");
+      } else if ((optText).Equals(Dafny.Sequence<Dafny.Rune>.UnicodeFromString(""))) {
+        return Dafny.Sequence<Dafny.Rune>.UnicodeFromString("panic!()");
+      } else {
+        return Dafny.Sequence<Dafny.Rune>.Concat(Dafny.Sequence<Dafny.Rune>.Concat(Dafny.Sequence<Dafny.Rune>.UnicodeFromString("panic!(\""), optText), Dafny.Sequence<Dafny.Rune>.UnicodeFromString("\")"));
+      }
+    }
     public Std.Wrappers._IOption<Dafny.ISequence<Dafny.Rune>> error {get; set;}
     public void __ctor(bool unicodeChars, DCOMP._IObjectType objectType)
     {
       (this)._UnicodeChars = unicodeChars;
       (this)._ObjectType = objectType;
       (this).error = Std.Wrappers.Option<Dafny.ISequence<Dafny.Rune>>.create_None();
+      if ((objectType).is_RawPointers) {
+        (this).error = Std.Wrappers.Option<Dafny.ISequence<Dafny.Rune>>.create_Some(Dafny.Sequence<Dafny.Rune>.UnicodeFromString("Raw pointers need to be wrapped in a newtype so that their equality has the semantics of Dafny (e.g. a class pointer and a trait pointer are equal), not Rust."));
+      }
     }
     public RAST._IMod GenModule(DAST._IModule mod, Dafny.ISequence<Dafny.ISequence<Dafny.Rune>> containingPath)
     {
@@ -1509,14 +1521,14 @@ namespace DCOMP {
                   _1285_rhs = Dafny.Sequence<Dafny.Rune>.Concat((_1286_hasMatchingField).dtor_value, Dafny.Sequence<Dafny.Rune>.UnicodeFromString(""));
                 }
               } else {
-                _1285_rhs = Dafny.Sequence<Dafny.Rune>.UnicodeFromString("panic!(\"field does not exist on this variant\")");
+                _1285_rhs = (this).UnreachablePanicIfVerified(Dafny.Sequence<Dafny.Rune>.UnicodeFromString("field does not exist on this variant"));
               }
               RAST._IMatchCase _1292_ctorMatch;
               _1292_ctorMatch = RAST.MatchCase.create(_1284_pattern, RAST.Expr.create_RawExpr(_1285_rhs));
               _1281_cases = Dafny.Sequence<RAST._IMatchCase>.Concat(_1281_cases, Dafny.Sequence<RAST._IMatchCase>.FromElements(_1292_ctorMatch));
             }
             if ((new BigInteger(((c).dtor_typeParams).Count)).Sign == 1) {
-              _1281_cases = Dafny.Sequence<RAST._IMatchCase>.Concat(_1281_cases, Dafny.Sequence<RAST._IMatchCase>.FromElements(RAST.MatchCase.create(Dafny.Sequence<Dafny.Rune>.Concat(_1257_datatypeName, Dafny.Sequence<Dafny.Rune>.UnicodeFromString("::_PhantomVariant(..)")), RAST.Expr.create_RawExpr(Dafny.Sequence<Dafny.Rune>.UnicodeFromString("panic!()")))));
+              _1281_cases = Dafny.Sequence<RAST._IMatchCase>.Concat(_1281_cases, Dafny.Sequence<RAST._IMatchCase>.FromElements(RAST.MatchCase.create(Dafny.Sequence<Dafny.Rune>.Concat(_1257_datatypeName, Dafny.Sequence<Dafny.Rune>.UnicodeFromString("::_PhantomVariant(..)")), RAST.Expr.create_RawExpr((this).UnreachablePanicIfVerified(Dafny.Sequence<Dafny.Rune>.UnicodeFromString(""))))));
             }
             RAST._IExpr _1293_methodBody;
             _1293_methodBody = RAST.Expr.create_Match(RAST.__default.self, _1281_cases);
@@ -1677,7 +1689,7 @@ namespace DCOMP {
       }
       if ((new BigInteger(((c).dtor_typeParams).Count)).Sign == 1) {
         Dafny.ISequence<RAST._IMatchCase> _1339_extraCases;
-        _1339_extraCases = Dafny.Sequence<RAST._IMatchCase>.FromElements(RAST.MatchCase.create(Dafny.Sequence<Dafny.Rune>.Concat(_1257_datatypeName, Dafny.Sequence<Dafny.Rune>.UnicodeFromString("::_PhantomVariant(..)")), RAST.Expr.create_RawExpr(Dafny.Sequence<Dafny.Rune>.UnicodeFromString("{panic!()}"))));
+        _1339_extraCases = Dafny.Sequence<RAST._IMatchCase>.FromElements(RAST.MatchCase.create(Dafny.Sequence<Dafny.Rune>.Concat(_1257_datatypeName, Dafny.Sequence<Dafny.Rune>.UnicodeFromString("::_PhantomVariant(..)")), RAST.Expr.create_RawExpr(Dafny.Sequence<Dafny.Rune>.Concat(Dafny.Sequence<Dafny.Rune>.Concat(Dafny.Sequence<Dafny.Rune>.UnicodeFromString("{"), (this).UnreachablePanicIfVerified(Dafny.Sequence<Dafny.Rune>.UnicodeFromString(""))), Dafny.Sequence<Dafny.Rune>.UnicodeFromString("}")))));
         _1315_printImplBodyCases = Dafny.Sequence<RAST._IMatchCase>.Concat(_1315_printImplBodyCases, _1339_extraCases);
         _1316_hashImplBodyCases = Dafny.Sequence<RAST._IMatchCase>.Concat(_1316_hashImplBodyCases, _1339_extraCases);
         _1317_coerceImplBodyCases = Dafny.Sequence<RAST._IMatchCase>.Concat(_1317_coerceImplBodyCases, _1339_extraCases);
@@ -5325,7 +5337,7 @@ namespace DCOMP {
                       goto after__ASSIGN_SUCH_THAT_2;
                     }
                   }
-                  throw new System.Exception("assign-such-that search produced no value (line 4389)");
+                  throw new System.Exception("assign-such-that search produced no value (line 4397)");
                 after__ASSIGN_SUCH_THAT_2: ;
                   _1892_allReadCloned = Dafny.Sequence<Dafny.Rune>.Concat(Dafny.Sequence<Dafny.Rune>.Concat(Dafny.Sequence<Dafny.Rune>.Concat(Dafny.Sequence<Dafny.Rune>.Concat(Dafny.Sequence<Dafny.Rune>.Concat(_1892_allReadCloned, Dafny.Sequence<Dafny.Rune>.UnicodeFromString("let ")), _1893_next), Dafny.Sequence<Dafny.Rune>.UnicodeFromString(" = ")), _1893_next), Dafny.Sequence<Dafny.Rune>.UnicodeFromString(".clone();\n"));
                   _1891_recIdents = Dafny.Set<Dafny.ISequence<Dafny.Rune>>.Difference(_1891_recIdents, Dafny.Set<Dafny.ISequence<Dafny.Rune>>.FromElements(_1893_next));
@@ -6614,7 +6626,7 @@ namespace DCOMP {
                   goto after__ASSIGN_SUCH_THAT_3;
                 }
               }
-              throw new System.Exception("assign-such-that search produced no value (line 4864)");
+              throw new System.Exception("assign-such-that search produced no value (line 4872)");
             after__ASSIGN_SUCH_THAT_3: ;
               if ((!object.Equals(selfIdent, DCOMP.SelfInfo.create_NoSelf())) && ((_2126_next).Equals(Dafny.Sequence<Dafny.Rune>.UnicodeFromString("_this")))) {
                 RAST._IExpr _2127_selfCloned;
